Prove that fib slow and fib fast implement fib

lean_proofs/LeanProofs/OpaqueFuncsInstance.lean
@@ -5,6 +5,8 @@ def map_append { t0 : Type } [Inhabited t0] (v1 v2 : Adt0 t0) := Adt0.mkadt0_0 (
 
 def map_slice { t0 : Type } [Inhabited t0] (v1 : Adt0 t0) (left right : Int) := Adt0.mkadt0_0 (fun x => if 0 <= x ∧ x < (right - left) then v1.fld0_0 (x + left) else default) (if right - left < 0 then 0 else right - left)
 
+def fib_rec (n : Nat) : Nat := if n ≤ 1 then 1 else fib_rec (n - 1) + fib_rec (n - 2)
+
 instance : FluxOpaqueFuncs where
   svec_default_elem := default
   svec_empty_seq { t0 : Type } [Inhabited t0] := fun _ => default
@@ -16,3 +18,4 @@ instance : FluxOpaqueFuncs where
   svec2_vseq_pop := List.tail
   svec2_vseq_set := fun l p e => List.set l (List.length l - p - 1).natAbs e
   svec2_vseq_len := Int.ofNat ∘ List.length
+  fib_fib (n : Int) := fib_rec n.natAbs
