lean_proofs/LeanProofs/Lib.lean
@@ -5,8 +5,8 @@ def BitVec_uge { n : Nat } (x y : BitVec n) := (BitVec.ult x y).not
 def BitVec_sge { n : Nat } (x y : BitVec n) := (BitVec.slt x y).not
 def BitVec_ugt { n : Nat } (x y : BitVec n) := (BitVec.ule x y).not
 def BitVec_sgt { n : Nat } (x y : BitVec n) := (BitVec.sle x y).not
-def SmtMap (Key Val : Type) [Inhabited Key] [BEq Key] [Inhabited Val] : Type := Key -> Val
-def SmtMap_default { Key Val: Type } (v : Val) [Inhabited Key] [BEq Key] [Inhabited Val] : SmtMap Key Val := fun _ => v
-def SmtMap_store { Key Val : Type } [Inhabited Key] [BEq Key] [Inhabited Val] (m : SmtMap Key Val) (k : Key) (v : Val) : SmtMap Key Val :=
+def SmtMap (t0 t1 : Type) [Inhabited t0] [BEq t0] [Inhabited t1] : Type := t0 -> t1
+def SmtMap_default { t0 t1: Type } (v : t1) [Inhabited t0] [BEq t0] [Inhabited t1] : SmtMap t0 t1 := fun _ => v
+def SmtMap_store { t0 t1 : Type } [Inhabited t0] [BEq t0] [Inhabited t1] (m : SmtMap t0 t1) (k : t0) (v : t1) : SmtMap t0 t1 :=
   fun x => if x == k then v else m x
-def SmtMap_select { Key Val : Type } [Inhabited Key] [BEq Key] [Inhabited Val] (m : SmtMap Key Val) (k : Key) := m k
+def SmtMap_select { t0 t1 : Type } [Inhabited t0] [BEq t0] [Inhabited t1] (m : SmtMap t0 t1) (k : t0) := m k
