lean_proofs/LeanProofs/SharedTheorems.lean
@@ -8,3 +8,4 @@ theorem svec2_vseq_get_eq { t0 : Type } [i: Inhabited t0] : @svec2_vseq_get t0 i
 theorem svec2_vseq_set_eq { t0 : Type } [i: Inhabited t0] : @svec2_vseq_set t0 i = fun l p e => l.set (l.length - p - 1).natAbs e := rfl
 theorem svec2_vseq_push_eq { t0 : Type } [i: Inhabited t0] : @svec2_vseq_push t0 i = flip List.cons := rfl
 theorem svec2_vseq_len_eq { t0 : Type } [i: Inhabited t0] : @svec2_vseq_len t0 i = Int.ofNat ∘ List.length := rfl
+theorem fib_fib_eq (n : Int) : fib_fib n = fib_rec n.natAbs := by rfl
